tests/lean/doErrorMsg.lean
@@ -25,5 +25,8 @@ def g3 : ExceptT String (StateT Nat Id) String := do
 
 example : Nat := Id.run do
   let mut n : Nat := 0
+  n := false
+  n : Char := false
   (n, _) := (false, false)
+  ((n : Char), _) := (false, false)
   n
