tests/lean/run/wf_preprocess.lean
@@ -209,21 +209,18 @@ theorem MTree.size.eq_1.{u_1} : ∀ {α : Type u_1} (t : MTree α),
   t.size =
     (have s := 1;
       do
-      let r ←
-        forIn t.cs s fun css r =>
-            have s := r;
+      let __s ←
+        forIn t.cs s fun css __s =>
+            have s := __s;
             do
-            let r ←
-              forIn css s fun c r =>
-                  have s := r;
+            let __s ←
+              forIn css s fun c __s =>
+                  have s := __s;
                   have s := s + c.size;
-                  do
-                  pure PUnit.unit
                   pure (ForInStep.yield s)
-            have s : Nat := r
-            pure PUnit.unit
+            have s : Nat := __s
             pure (ForInStep.yield s)
-      have s : Nat := r
+      have s : Nat := __s
       pure s).run
 -/
 #guard_msgs in
